Add full annotations

operational_semantics/operational_semantics.v
@@ -9,49 +9,48 @@ Inductive step : comp -> comp -> Prop :=
     step 
       (ProdMatch (Pair v1 v2) c)
       (c_subs2_out c v1 v2)
-| Step_MatchLeft v c1 c2:
+| Step_MatchLeft A B v c1 c2:
     step 
-      (SumMatch (Left v) c1 c2)
+      (SumMatch (Left A B v) c1 c2)
       (c_subs_out c1 v)
-| Step_MatchRight v c1 c2:
+| Step_MatchRight A B v c1 c2:
     step 
-      (SumMatch (Right v) c1 c2)
+      (SumMatch (Right A B v) c1 c2)
       (c_subs_out c2 v)
-| Step_MatchNil c1 c2:
+| Step_MatchNil A c1 c2:
     step 
-      (ListMatch Nil c1 c2)
+      (ListMatch (Nil A) c1 c2)
       c1
 | Step_MatchCons v vs c1 c2:
     step 
       (ListMatch (Cons v vs) c1 c2)
       (c_subs2_out c2 v vs)
-| Step_AppFun c v:
-    step (App (Fun c) v) (c_subs_out c v)
-| Step_LetRec c1 c2:
+| Step_AppFun A c v:
+    step (App (Fun A c) v) (c_subs_out c v)
+| Step_LetRecStep A C c1 c2:
     step
-      (LetRec c1 c2)
-      (c_subs_out c2 (Fun (LetRec (c_shift c1 1 2) c1)))
+      (LetRec A C c1 c2)
+      (c_subs_out c2 (Fun A (LetRec A C (c_shift c1 1 2) c1)))
 | Step_DoStep c1 c1' c2:
     step c1 c1' ->
     step (Do c1 c2) (Do c1' c2)
 | Step_DoRet v c:
     step (Do (Ret v) c) (c_subs_out c v)
-| Step_DoOp op v c1 c2:
+| Step_DoOp op A B v c1 c2:
     step
-      (Do (Op op v c1) c2)
-      (Op op v (Do c1 (c_shift c2 1 1)))
+      (Do (Op op A B v c1) c2)
+      (Op op A B v (Do c1 (c_shift c2 1 1)))
 | Step_HandleStep v c c' :
     step c c' ->
     step (Handle v c) (Handle v c')
-| Step_HandleRet c_r h v :
+| Step_HandleRet A c_r h v :
     step
-      (Handle (Handler c_r h) (Ret v))
+      (Handle (Handler A c_r h) (Ret v))
       (c_subs_out c_r v)
-| Step_HandleOp c_r h op v c_k c_op :
+| Step_HandleOp A c_r h op Aop Bop v c_k c_op :
     get_case h op = Some c_op ->
     step
-      (Handle (Handler c_r h) (Op op v c_k))
-      (c_subs2_out c_op
-        (Fun (Handle (v_shift (Handler c_r h) 1 0) c_k))
-        v )
+      (Handle (Handler A c_r h) (Op op Aop Bop v c_k))
+      (c_subs2_out c_op v
+        (Fun Bop (Handle (v_shift (Handler A c_r h) 1 0) c_k)) )
 .
