type_system/declarational.v
@@ -9,55 +9,55 @@ Require Export syntax subtyping substitution.
 (* ==================== Template Handling ==================== *)
 
 (* We increase context length so that we don't have to shift h. *)
-Fixpoint handle_t Γ_len Z_len h T :=
+Fixpoint handle_t D Γ_len Z_len h T :=
   match T with
   | TApp n v => App (Var (Γ_len+n)) v
-  | TAbsurd v => Absurd v
+  | TAbsurd v => Absurd D v
   | TProdMatch v T => 
-      ProdMatch v (handle_t (2+Γ_len) Z_len h T)
+      ProdMatch v (handle_t D (2+Γ_len) Z_len h T)
   | TSumMatch v T1 T2 => 
       SumMatch v
-        (handle_t (1+Γ_len) Z_len h T1) 
-        (handle_t (1+Γ_len) Z_len h T2)
+        (handle_t D (1+Γ_len) Z_len h T1) 
+        (handle_t D (1+Γ_len) Z_len h T2)
   | TListMatch v T1 T2 =>
       ListMatch v
-        (handle_t Γ_len Z_len h T1)
-        (handle_t (2+Γ_len) Z_len h T2)
+        (handle_t D Γ_len Z_len h T1)
+        (handle_t D (2+Γ_len) Z_len h T2)
   | TDo c T =>
-      Do c (handle_t (1+Γ_len) Z_len h T)
-  | TOp op v T =>
+      Do c (handle_t D (1+Γ_len) Z_len h T)
+  | TOp op A B v T =>
       match get_case h op with 
       | Some c_op =>
           c_subs2_out (c_shift c_op (Γ_len + Z_len) 2) 
-              (Fun (handle_t (1+Γ_len) Z_len h T)) v
+            v (Fun B (handle_t D (1+Γ_len) Z_len h T))
       | None => 
           (* You shouldn't be here *)
-          Op op v (handle_t (1+Γ_len) Z_len h T) 
+          Op op A B v (handle_t D (1+Γ_len) Z_len h T) 
       end
   end.
 
 
-Fixpoint tmpl_to_comp Γ_len T :=
+Fixpoint tmpl_to_comp C Γ_len T :=
   match T with
   | TApp n v => App (Var (Γ_len+n)) v
-  | TAbsurd v => Absurd v
+  | TAbsurd v => Absurd C v
   | TProdMatch v T => 
-      ProdMatch v (tmpl_to_comp (2+Γ_len) T)
+      ProdMatch v (tmpl_to_comp C (2+Γ_len) T)
   | TSumMatch v T1 T2 => 
       SumMatch v
-        (tmpl_to_comp (1+Γ_len) T1) 
-        (tmpl_to_comp (1+Γ_len) T2)
+        (tmpl_to_comp C (1+Γ_len) T1) 
+        (tmpl_to_comp C (1+Γ_len) T2)
   | TListMatch v T1 T2 => 
       ListMatch v
-        (tmpl_to_comp Γ_len T1) 
-        (tmpl_to_comp (2+Γ_len) T2)
+        (tmpl_to_comp C Γ_len T1) 
+        (tmpl_to_comp C (2+Γ_len) T2)
   | TDo c T =>
-      Do c (tmpl_to_comp (1+Γ_len) T)
-  | TOp op v T =>
-      Op op v (tmpl_to_comp (1+Γ_len) T)
+      Do c (tmpl_to_comp C (1+Γ_len) T)
+  | TOp op A B v T =>
+      Op op A B v (tmpl_to_comp C (1+Γ_len) T)
   end.
 
-(* ==================== Wellformed Judgements ==================== *)
+(* ==================== Welljudged Judgements ==================== *)
 
 Inductive wf_vtype : vtype -> Prop :=
 | WfTyUnit : wf_vtype TyUnit 
@@ -109,10 +109,13 @@ with wf_t : ctx -> tctx -> tmpl -> sig -> Prop :=
     has_ctype Γ c (CTy A SigØ EqsØ) ->
     wf_t (CtxU Γ A) Z T Σ ->
     wf_t  Γ Z (TDo c T) Σ
-| WfTOp Γ Z op v T Aop Bop Σ :
-    get_op_type Σ op = Some (Aop, Bop) -> has_vtype Γ v Aop ->
+| WfTOp Γ Z op Aop Bop v T A B Σ :
+    get_op_type Σ op = Some (A, B) -> 
+    vsubtype Aop A -> vsubtype B Bop ->
+    wf_vtype Aop -> wf_vtype Bop ->
+    has_vtype Γ v Aop ->
     wf_t (CtxU Γ Bop) Z T Σ ->
-    wf_t Γ Z (TOp op v T) Σ
+    wf_t Γ Z (TOp op Aop Bop v T) Σ
 
 with wf_eqs : eqs -> sig -> Prop :=
 | WfEqsØ Σ : wf_eqs EqsØ Σ
@@ -120,6 +123,7 @@ with wf_eqs : eqs -> sig -> Prop :=
     wf_eqs E Σ -> wf_ctx Γ -> wf_tctx Z -> wf_sig Σ ->
     wf_t Γ Z T1 Σ -> wf_t Γ Z T2 Σ -> 
     wf_eqs (EqsU E Γ Z T1 T2) Σ
+
 
 (* ==================== Type Judgements ==================== *)
 
@@ -143,24 +147,24 @@ with has_vtype' : ctx -> val -> vtype -> Prop :=
     has_vtype' Γ (Pair v1 v2) (TyProd A B)
 | TypeLeft Γ v A B :
     has_vtype Γ v A ->
-    has_vtype' Γ (Left v) (TySum A B)
+    has_vtype' Γ (Left A B v) (TySum A B)
 | TypeRight Γ v A B :
     has_vtype Γ v B ->
-    has_vtype' Γ (Right v) (TySum A B)
+    has_vtype' Γ (Right A B v) (TySum A B)
 | TypeNil Γ A :
-    has_vtype' Γ Nil (TyList A)
+    has_vtype' Γ (Nil A) (TyList A)
 | TypeCons Γ v vs A :
     has_vtype Γ v A ->
     has_vtype Γ vs (TyList A) ->
     has_vtype' Γ (Cons v vs) (TyList A)
 | TypeFun Γ c A C :
     has_ctype (CtxU Γ A) c C ->
-    has_vtype' Γ (Fun c) (TyFun A C)
+    has_vtype' Γ (Fun A c) (TyFun A C)
 | TypeHandler Γ cr h A Σ E D :
     has_ctype (CtxU Γ A) cr D ->
     has_htype Γ h Σ D -> 
     respects Γ h Σ D E ->
-    has_vtype' Γ (Handler cr h) (TyHandler (CTy A Σ E) D)
+    has_vtype' Γ (Handler A cr h) (TyHandler (CTy A Σ E) D)
 | TypeVSubsume Γ v A A' :
     has_vtype Γ v A ->
     vsubtype A A' -> 
@@ -178,7 +182,7 @@ with has_ctype' : ctx -> comp -> ctype -> Prop :=
     has_ctype' Γ (Ret v) (CTy A SigØ EqsØ)
 | TypeAbsurd Γ v C :
     has_vtype Γ v TyEmpty -> 
-    has_ctype' Γ (Absurd v) C
+    has_ctype' Γ (Absurd C v) C
 | TypeProdMatch Γ v A B c C :
     has_vtype Γ v (TyProd A B) ->
     has_ctype (CtxU (CtxU Γ A) B) c C ->
@@ -208,12 +212,13 @@ with has_ctype' : ctx -> comp -> ctype -> Prop :=
 | TypeLetRec Γ A C c1 c2 D:
     has_ctype (CtxU (CtxU Γ A) (TyFun A C)) c1 C ->
     has_ctype (CtxU Γ (TyFun A C)) c2 D ->
-    has_ctype' Γ (LetRec c1 c2) D
-| TypeOp Γ op v c Aop Bop A Σ E :
-    get_op_type Σ op = Some (Aop, Bop) ->
+    has_ctype' Γ (LetRec A C c1 c2) D
+| TypeOp Γ op v c Aop Bop Aop' Bop' A Σ E :
+    get_op_type Σ op = Some (Aop', Bop') -> 
+    vsubtype Aop Aop' -> vsubtype Bop' Bop ->
     has_vtype Γ v Aop ->
     has_ctype (CtxU Γ Bop) c (CTy A Σ E) ->
-    has_ctype' Γ (Op op v c) (CTy A Σ E)
+    has_ctype' Γ (Op op Aop Bop v c) (CTy A Σ E)
 | TypeCSubsume Γ c C C' :
     has_ctype Γ c C -> 
     csubtype C C' -> 
@@ -226,11 +231,11 @@ with has_htype : ctx -> hcases -> sig -> ctype -> Prop :=
     has_htype Γ h Σ D
 
 with has_htype' : ctx -> hcases -> sig -> ctype -> Prop :=
-| TypeCasesØ Γ D : has_htype' Γ CasesØ SigØ D
-| TypeCasesU Γ h op cop Aop Bop Σ D :
+| TypeCasesØ Γ D : has_htype' Γ (CasesØ D) SigØ D
+| TypeCasesU Γ h op c A B Σ D :
     has_htype Γ h Σ D ->
-    has_ctype (CtxU (CtxU Γ (TyFun Bop D)) Aop) cop D ->
-    has_htype' Γ (CasesU h op cop) (SigU Σ op Aop Bop) D
+    has_ctype (CtxU (CtxU Γ A) (TyFun B D)) c D ->
+    has_htype' Γ (CasesU h op A B c) (SigU Σ op A B) D
 
 (* ==================== Logic Judgements ==================== *)
 
@@ -245,8 +250,8 @@ with respects' : ctx -> hcases -> sig -> ctype -> eqs -> Prop :=
 | RespectEqsU Γ h Σ D E Γ' Z T1 T2 :
     respects Γ' h Σ D E -> 
     ceq D (join_ctxs (join_ctxs Γ' (tctx_to_ctx Z D)) Γ)
-      (handle_t (ctx_len Γ) (tctx_len Z) h T1) 
-      (handle_t (ctx_len Γ) (tctx_len Z) h T2) ->
+      (handle_t D (ctx_len Γ) (tctx_len Z) h T1) 
+      (handle_t D (ctx_len Γ) (tctx_len Z) h T2) ->
     respects' Γ' h Σ D (EqsU E Γ Z T1 T2)
 
 with veq : vtype -> ctx -> val -> val -> Prop := 
@@ -263,8 +268,8 @@ with veq': vtype -> ctx -> val -> val -> Prop :=
     veq A Γ v1 v2 -> veq A Γ v2 v3 -> 
     veq' A Γ v1 v3
 | VeqVar i A A' Γ :
-    get_vtype Γ i = Some A' ->
-    vsubtype A' A ->
+    get_vtype Γ i = Some A' -> 
+    vsubtype A' A -> (* Extra subtyping *)
     veq' A Γ (Var i) (Var i)
 | VeqUnit Γ:
     veq' TyUnit Γ Unit Unit
@@ -274,30 +279,36 @@ with veq': vtype -> ctx -> val -> val -> Prop :=
     veq A Γ v1 v1' ->
     veq B Γ v2 v2' -> 
     veq' (TyProd A B) Γ (Pair v1 v2) (Pair v1' v2')
-| VeqLeft A B Γ v v' :
+| VeqLeft A A1 A2 B B1 B2 Γ v v' :
     veq A Γ v v' ->
-    veq' (TySum A B) Γ (Left v) (Left v')
-| VeqRight A B Γ v v' :
+    vsubtype A1 A -> vsubtype A2 A -> vsubtype B1 B -> vsubtype B2 B ->
+    veq' (TySum A B) Γ (Left A1 B1 v) (Left A2 B2 v')
+| VeqRight A A1 A2 B B1 B2 Γ v v' :
     veq B Γ v v' ->
-    veq' (TySum A B) Γ (Right v) (Right v')
-| VeqNil A Γ :
-    veq' (TyList A) Γ Nil Nil
+    vsubtype A1 A -> vsubtype A2 A -> vsubtype B1 B -> vsubtype B2 B ->
+    veq' (TySum A B) Γ (Right A1 B1 v) (Right A2 B2 v')
+| VeqNil A A1 A2 Γ :
+    vsubtype A1 A -> vsubtype A2 A ->
+    veq' (TyList A) Γ (Nil A1) (Nil A2)
 | VeqCons A Γ v v' vs vs':
     veq A Γ v v' ->
     veq (TyList A) Γ vs vs' ->
     veq' (TyList A) Γ (Cons v vs) (Cons v' vs')
-| VeqFun A C Γ c c':
+| VeqFun A A1 A2 C Γ c c':
     ceq C (CtxU Γ A) c c' ->
-    veq' (TyFun A C) Γ (Fun c) (Fun c')
-| VeqHandler A Σ E D D' Γ c c' h h':
+    vsubtype A A1 -> vsubtype A A2 ->
+    veq' (TyFun A C) Γ (Fun A1 c) (Fun A2 c')
+| VeqHandler A A1 A2 Σ E D D' Γ c c' h h':
     ceq D (CtxU Γ A) c c' ->
     heq Σ D' Γ h h' ->
-    csubtype D' D ->
-    veq' (TyHandler (CTy A Σ E) D) Γ (Handler c h) (Handler c' h')
+    vsubtype A A1 -> vsubtype A A2 -> csubtype D' D -> (* Extra subtyping *)
+    veq' (TyHandler (CTy A Σ E) D) Γ (Handler A1 c h) (Handler A2 c' h')
 | ηUnit Γ v:
     veq' TyUnit Γ v Unit
-| ηFun A C Γ f:
-    veq' (TyFun A C) Γ (Fun (App (v_shift f 1 0) (Var 0))) f
+| ηFun A A' C Γ f:
+    (* Extra subtyping *)
+    vsubtype A A' ->
+    veq' (TyFun A C) Γ (Fun A' (App (v_shift f 1 0) (Var 0))) f
 
 
 with ceq : ctype -> ctx -> comp -> comp -> Prop := 
@@ -317,8 +328,9 @@ with ceq' : ctype -> ctx -> comp -> comp -> Prop :=
 | CeqRet A Σ E Γ v v' : 
     veq A Γ v v' -> 
     ceq' (CTy A Σ E) Γ (Ret v) (Ret v')
-| CeqAbsurd C Γ v v' :
-    ceq' C Γ (Absurd v) (Absurd v')
+| CeqAbsurd C C1 C2 Γ v v' :
+    csubtype C1 C -> csubtype C2 C ->
+    ceq' C Γ (Absurd C1 v) (Absurd C2 v')
 | CeqProdMatch Γ C v v' A B c c':
     veq (TyProd A B) Γ v v' ->
     ceq C (CtxU (CtxU Γ A) B) c c' ->
@@ -348,65 +360,69 @@ with ceq' : ctype -> ctx -> comp -> comp -> Prop :=
 | CeqLetRec Γ c1 c1' c2 c2' A C D:
     ceq C (CtxU (CtxU Γ A) (TyFun A C)) c1 c1' ->
     ceq D (CtxU Γ (TyFun A C)) c2 c2' ->
-    ceq' D Γ (LetRec c1 c2) (LetRec c1' c2')
-| CeqOp Γ op v v' c c' Aop Bop A Σ E:
+    ceq' D Γ (LetRec A C c1 c2) (LetRec A C c1' c2')
+| CeqOp Γ op v v' c c' A A' Aop B B' Bop Ac Σ E:
     get_op_type Σ op = Some (Aop, Bop) ->
+    vsubtype A Aop -> vsubtype A' Aop -> vsubtype Bop B -> vsubtype Bop B' ->
     veq Aop Γ v v' ->
-    ceq (CTy A Σ E) (CtxU Γ Bop) c c' ->
-    ceq' (CTy A Σ E) Γ (Op op v c) (Op op v' c')
-| OOTB A Σ E Γ' I Γ Z T1 T2 c1 c2:
+    ceq (CTy Ac Σ E) (CtxU Γ Bop) c c' ->
+    ceq' (CTy Ac Σ E) Γ (Op op A B v c) (Op op A' B' v' c')
+| OOTB A Σ E C Γ' I Γ Z T1 T2 c1 c2:
+    (* Extra subtyping *)
+    csubtype (CTy A Σ E) C -> wf_ctype (CTy A Σ E) ->
     has_eq E Γ Z T1 T2 ->
     wf_inst Γ' I (join_ctxs (tctx_to_ctx Z (CTy A Σ E)) Γ) ->
-    c_inst (tmpl_to_comp (ctx_len Γ) T1) I = c1 ->
-    c_inst (tmpl_to_comp (ctx_len Γ) T2) I = c2 ->
-    ceq' (CTy A Σ E) Γ' c1 c2
+    c_inst (tmpl_to_comp (CTy A Σ E) (ctx_len Γ) T1) I = c1 ->
+    c_inst (tmpl_to_comp (CTy A Σ E) (ctx_len Γ) T2) I = c2 ->
+    ceq' C Γ' c1 c2
 | βMatchPair v1 v2 c C Γ: 
     ceq' C Γ
       (ProdMatch (Pair v1 v2) c) 
       (c_subs2_out c v1 v2)
-| βMatchLeft v c1 c2 C Γ:
+| βMatchLeft v c1 c2 C A B Γ:
     ceq' C Γ
-      (SumMatch (Left v) c1 c2)
+      (SumMatch (Left A B v) c1 c2)
       (c_subs_out c1 v)
-| βMatchRight v c1 c2 C Γ:
+| βMatchRight v c1 c2 C A B Γ:
     ceq' C Γ 
-      (SumMatch (Right v) c1 c2)
+      (SumMatch (Right A B v) c1 c2)
       (c_subs_out c2 v)
-| βMatchNil c1 c2 C Γ:
+| βMatchNil c1 c2 A C Γ:
     ceq' C Γ
-      (ListMatch Nil c1 c2)
+      (ListMatch (Nil A) c1 c2)
       c1
 | βMatchCons v vs c1 c2 C Γ:
     ceq' C Γ
       (ListMatch (Cons v vs) c1 c2)
       (c_subs2_out c2 v vs)
-| βApp c v C Γ:
-    ceq' C Γ (App (Fun c) v) (c_subs_out c v)
-| βLetRec c1 c2 C Γ:
-    ceq' C Γ
-      (LetRec c1 c2)
-      (c_subs_out c2 (Fun (LetRec (c_shift c1 1 2) c1)))
+| βApp c v A C Γ:
+    ceq' C Γ (App (Fun A c) v) (c_subs_out c v)
+| βLetRec c1 c2 A C D Γ:
+    ceq' D Γ
+      (LetRec A C c1 c2)
+      (c_subs_out c2 (Fun A (LetRec A C (c_shift c1 1 2) c1)))
 | βDoRet v c C Γ:
     ceq' C Γ (Do (Ret v) c) (c_subs_out c v)
-| βDoOp op v c1 c2 C Γ:
+| βDoOp op v c1 c2 Aop Bop C Γ:
     ceq' C Γ
-      (Do (Op op v c1) c2)
-      (Op op v (Do c1 (c_shift c2 1 1)))
-| βHandleRet c_r h v C Γ:
+      (Do (Op op Aop Bop v c1) c2)
+      (Op op Aop Bop v (Do c1 (c_shift c2 1 1)))
+| βHandleRet c_r h v A C Γ:
     ceq' C Γ
-      (Handle (Handler c_r h) (Ret v))
+      (Handle (Handler A c_r h) (Ret v))
       (c_subs_out c_r v)
-| βHandleOp c_r h op v c_k c_op C Γ:
+| βHandleOp c_r h op Aop Bop v c_k c_op A C Γ:
     get_case h op = Some c_op ->
     ceq' C Γ
-      (Handle (Handler c_r h) (Op op v c_k))
+      (Handle (Handler A c_r h) (Op op Aop Bop v c_k))
       (c_subs2_out c_op
-        (Fun (Handle (v_shift (Handler c_r h) 1 0) c_k))
-        v )
-| ηEmpty Γ v n c C:
+        v (Fun Bop (Handle (v_shift (Handler A c_r h) 1 0) c_k)) )
+| ηEmpty Γ v n c C C':
+    (* Extra subtyping *)
     n <= ctx_len Γ ->
+    csubtype C C' ->
     has_ctype (ctx_insert Γ n (TyEmpty)) c C ->
-    ceq' C Γ (c_subs c n v) (Absurd v)
+    ceq' C' Γ (c_subs c n v) (Absurd C v)
 | ηPair Γ v n c C A B:
     n <= ctx_len Γ ->
     has_ctype (ctx_insert Γ n (TyProd A B)) c C ->
@@ -417,14 +433,14 @@ with ceq' : ctype -> ctx -> comp -> comp -> Prop :=
     has_ctype (ctx_insert Γ n (TySum A B)) c C ->
     ceq' C Γ (c_subs c n v) 
       (SumMatch v 
-        (c_subs (c_shift c 1 0) (1+n) (Left (Var 0))) 
-        (c_subs (c_shift c 1 0) (1+n) (Right (Var 0))))
+        (c_subs (c_shift c 1 0) (1+n) (Left A B (Var 0))) 
+        (c_subs (c_shift c 1 0) (1+n) (Right A B (Var 0))))
 | ηList Γ v n c C A:
     n <= ctx_len Γ ->
     has_ctype (ctx_insert Γ n (TyList A)) c C ->
     ceq' C Γ (c_subs c n v) 
       (ListMatch v 
-        (c_subs c n Nil) 
+        (c_subs c n (Nil A)) 
         (c_subs (c_shift c 2 0) (2+n) (Cons (Var 1) (Var 0))))
 | ηDo Γ c C:
     ceq' C Γ (Do c (Ret (Var 0))) c
@@ -442,7 +458,7 @@ with heq' : sig -> ctype -> ctx -> hcases -> hcases -> Prop :=
 | HeqSigU Σ op A B D Γ h1 c1 h2 c2:
     get_case h1 op = Some c1 ->
     get_case h2 op = Some c2 ->
-    ceq D (CtxU (CtxU Γ (TyFun B D)) A) c1 c2 ->
+    ceq D (CtxU (CtxU Γ A) (TyFun B D)) c1 c2 ->
     heq Σ D Γ h1 h2 ->
     heq' (SigU Σ op A B) D Γ h1 h2
 
